memmgr/spec_malloc.v
@@ -1624,17 +1624,15 @@ Definition size2bin_spec :=
 
 Definition list_from_block_spec :=
  DECLARE _list_from_block
-  WITH s: Z, p: val, r: val, rlen: nat, b: Z
-  PRE [ _s OF tuint, _p OF tptr tschar, _r OF tptr tvoid ]    
-     PROP( s = bin2sizeZ b /\ 
-(* WORD <= s <= bin2sizeZ(BINS-1) /\ *)
-malloc_compatible BIGBLOCK p ) 
-     LOCAL (temp _s (Vptrofs (Ptrofs.repr s)); temp _p p; temp _r r)
-     SEP ( memory_block Tsh BIGBLOCK p; mmlist s rlen r nullval )
+  WITH s: Z, p: val, tl: val, tlen: nat, b: Z
+  PRE [ _s OF tuint, _p OF tptr tschar, _tl OF tptr tvoid ]    
+     PROP( 0 <= b < BINS /\ s = bin2sizeZ b /\ malloc_compatible BIGBLOCK p ) 
+     LOCAL (temp _s (Vptrofs (Ptrofs.repr s)); temp _p p; temp _tl tl)
+     SEP ( memory_block Tsh BIGBLOCK p; mmlist s tlen tl nullval )
   POST [ tptr tvoid ] EX res:_,
      PROP() 
      LOCAL(temp ret_temp res)
-     SEP ( mmlist s (Z.to_nat(chunks_from_block (size2binZ s)) + rlen) res nullval * TT ).
+     SEP ( mmlist s (Z.to_nat(chunks_from_block (size2binZ s)) + tlen) res nullval * TT ).
 
 
 (* The postcondition describes the list returned, together with
